src/Utils/Monad.v
@@ -27,6 +27,11 @@ Notation "p <?- e ; b" :=
   (Mbind (fun x => match x with p => b | _ => Mfail end) e)
     (in custom monadic_do at level 90, left associativity, p pattern at level 0, e constr, b custom monadic_do).
 
+
+Notation "'let' p := e ; b" :=
+  (let p := e in b)
+    (in custom monadic_do at level 90, left associativity, p pattern at level 0, e constr, b custom monadic_do).
+
 Notation "'ret' e" := (Mret e) (in custom monadic_do at level 90, e constr).
 
 (*Notation "e" := (e) (in custom monadic_do at level 80, e constr at level 80).*)
