README.md
@@ -5,12 +5,13 @@
   + clear old files in other dirs
   + move IndependentJudgment out of ICore
   + rename/expand or at least roadmap Decidable
-* Fully switch to independent judgment (no elab) for all existing languages
+* Fully switch to independent judgment (no elab) for all existing languages? (currently reconsidering)
 * Relate independent judgment to original via elab to port theorems (or is it easier to replicate them?)
 * Clear admits in Decidable
 * Extend Decidable to work for compilers when possible
+* Fix reduction lemma to be sound
 * Improve automation to be consistent across all uses
-* determine whether there is an issue w/ current lax typing on le judgments
-* Either: remove IExp and use Exp for everything
+* determine whether there is an issue w/ current lax typing on le judgments (probably)
+* Either: remove IExp and use Exp for everything (this one I think)
 * Or: implement equality? and fill admits in subst lemmas for IExp
 * fill admits (or remove lemmas) for identity operation in Tactics
